feat(Mutations): Storage changes for a better tomorrow

AwsCryptographicMaterialProviders/runtimes/java/src/main/smithy-generated/software/amazon/cryptography/keystore/IKeyStorageInterface.java
@@ -3,8 +3,8 @@
 // Do not modify this file. This file is machine generated, and any changes to it will be overwritten.
 package software.amazon.cryptography.keystore;
 
-import software.amazon.cryptography.keystore.model.DeleteMutationLockAndIndexInput;
-import software.amazon.cryptography.keystore.model.DeleteMutationLockAndIndexOutput;
+import software.amazon.cryptography.keystore.model.DeleteMutationInput;
+import software.amazon.cryptography.keystore.model.DeleteMutationOutput;
 import software.amazon.cryptography.keystore.model.GetEncryptedActiveBranchKeyInput;
 import software.amazon.cryptography.keystore.model.GetEncryptedActiveBranchKeyOutput;
 import software.amazon.cryptography.keystore.model.GetEncryptedBeaconKeyInput;
@@ -15,14 +15,10 @@ import software.amazon.cryptography.keystore.model.GetItemsForInitializeMutation
 import software.amazon.cryptography.keystore.model.GetItemsForInitializeMutationOutput;
 import software.amazon.cryptography.keystore.model.GetKeyStorageInfoInput;
 import software.amazon.cryptography.keystore.model.GetKeyStorageInfoOutput;
-import software.amazon.cryptography.keystore.model.GetMutationLockAndIndexInput;
-import software.amazon.cryptography.keystore.model.GetMutationLockAndIndexOutput;
-import software.amazon.cryptography.keystore.model.GetMutationLockInput;
-import software.amazon.cryptography.keystore.model.GetMutationLockOutput;
+import software.amazon.cryptography.keystore.model.GetMutationInput;
+import software.amazon.cryptography.keystore.model.GetMutationOutput;
 import software.amazon.cryptography.keystore.model.QueryForVersionsInput;
 import software.amazon.cryptography.keystore.model.QueryForVersionsOutput;
-import software.amazon.cryptography.keystore.model.UpdateMutationIndexInput;
-import software.amazon.cryptography.keystore.model.UpdateMutationIndexOutput;
 import software.amazon.cryptography.keystore.model.WriteInitializeMutationInput;
 import software.amazon.cryptography.keystore.model.WriteInitializeMutationOutput;
 import software.amazon.cryptography.keystore.model.WriteMutatedVersionsInput;
@@ -34,12 +30,10 @@ import software.amazon.cryptography.keystore.model.WriteNewEncryptedBranchKeyVer
 
 public interface IKeyStorageInterface {
   /**
-   * Delete an existing Mutation Lock & Mutation Index.
+   * Delete an existing Mutation Commitment & Index.
    *
    */
-  DeleteMutationLockAndIndexOutput DeleteMutationLockAndIndex(
-    DeleteMutationLockAndIndexInput input
-  );
+  DeleteMutationOutput DeleteMutation(DeleteMutationInput input);
 
   /**
    * Get the ACTIVE branch key for encryption for an existing branch key.
@@ -73,7 +67,7 @@ public interface IKeyStorageInterface {
 
   /**
    * Gets the ACTIVE branch key and the beacon key,
-   * and looks for a Mutation Lock & Index,
+   * and looks for a Mutation Commitment & Index,
    * returning them if found.
    *
    */
@@ -90,22 +84,12 @@ public interface IKeyStorageInterface {
   GetKeyStorageInfoOutput GetKeyStorageInfo(GetKeyStorageInfoInput input);
 
   /**
-   * Check for Mutation Lock on a Branch Key ID.
+   * Check for Mutation Commitment on a Branch Key ID.
    * If one exists, returns the Mutation Lock.
    * Otherwise, returns nothing.
    *
    */
-  GetMutationLockOutput GetMutationLock(GetMutationLockInput input);
-
-  /**
-   * Check for Mutation Lock on a Branch Key ID.
-   * If one exists, returns the Mutation Lock.
-   * Otherwise, returns nothing.
-   *
-   */
-  GetMutationLockAndIndexOutput GetMutationLockAndIndex(
-    GetMutationLockAndIndexInput input
-  );
+  GetMutationOutput GetMutation(GetMutationInput input);
 
   /**
    * Query Storage for a page of version (decrypt only) items
@@ -115,18 +99,13 @@ public interface IKeyStorageInterface {
   QueryForVersionsOutput QueryForVersions(QueryForVersionsInput input);
 
   /**
-   * Updates a Mutation Index.
-   *
-   */
-  UpdateMutationIndexOutput UpdateMutationIndex(UpdateMutationIndexInput input);
-
-  /**
    * Atomically writes,
    * in the terminal state of a Mutation:
    * - new ACTIVE item
    * - version (decrypt only) for new ACTIVE
    * - beacon key
-   * Also writes the Mutation Lock & Index.
+   * - mutated Versions
+   * Also writes the Mutation Commitment & Index.
    *
    */
   WriteInitializeMutationOutput WriteInitializeMutation(
@@ -140,8 +119,7 @@ public interface IKeyStorageInterface {
    * conditioned on:
    * - every version already exsisting
    * - every version's enc has not changed
-   * - the original of a Mutation Lock commits to the original provided
-   * - the terminal of a Mutation Lock commits to the terminal provided
+   * - the Mutation Commitment has not changed
    *
    *
    */
